Present algorithm using variable p instead of the iteration count.
- I'd like to include the formalization in the paper (and this makes it easier to identify the corresponding part, w.r.t the informal algorithm.)

isabelle/CVM_Subsample/CVM_Abstract_Algorithm.thy
@@ -51,10 +51,6 @@ The part that is not going to be verified in this section, is the fact that the 
 most $n$ elements in the state $\chi$, because it is not unconditionally true, but will be ensured
 (by different means) for the concrete instantiations in the following sections.
 
-In contrast to the informal description (Algorithm~\ref{alg:cvm_abs}), the formalization keeps track
-of $k$ in its state, which is the number of subsampling operations, however this is an equivalent
-representation, because $p$ is then just $f^k$.
-
 An informal version of this proof is presented in Appendix~\ref{apx:informal_proof}.
 For important lemmas and theorems, we include a reference to the corresponding statement in the
 appendix.\<close>
@@ -71,7 +67,7 @@ begin
 unbundle no_vec_syntax
 
 record 'a state =
-  state_k :: nat
+  state_p :: real
   state_\<chi> :: \<open>'a set\<close>
 
 datatype 'a run_state = FinalState \<open>'a list\<close> | IntermState \<open>'a list\<close> \<open>'a\<close>
@@ -102,16 +98,16 @@ begin
 
 text \<open>Line 1 of Algorithm~\ref{alg:cvm_abs}:\<close>
 definition initial_state :: \<open>'a state\<close> where
-  \<open>initial_state \<equiv> \<lparr>state_k = 0, state_\<chi> = {}\<rparr>\<close>
+  \<open>initial_state \<equiv> \<lparr>state_p = 1, state_\<chi> = {}\<rparr>\<close>
 
 text \<open>Lines 3--7:\<close>
 definition step_1 :: \<open>'a \<Rightarrow> 'a state \<Rightarrow> 'a state pmf\<close> where
   \<open>step_1 x \<sigma> =
     do {
-      let k = state_k \<sigma>;
+      let p = state_p \<sigma>;
       let \<chi> = state_\<chi> \<sigma>;
 
-      insert_x_into_\<chi> \<leftarrow> bernoulli_pmf (f ^ k);
+      insert_x_into_\<chi> \<leftarrow> bernoulli_pmf p;
 
       let \<chi> = (
         if insert_x_into_\<chi>
@@ -125,13 +121,13 @@ definition step_1 :: \<open>'a \<Rightarrow> 'a state \<Rightarrow> 'a state pmf
 text \<open>Lines 8--10:\<close>
 definition step_2 :: \<open>'a state \<Rightarrow> 'a state pmf\<close> where
   \<open>step_2 \<sigma> = do {
-    let k = state_k \<sigma>;
+    let p = state_p \<sigma>;
     let \<chi> = state_\<chi> \<sigma>;
 
     if card \<chi> = thresh
     then do {
       \<chi> \<leftarrow> subsample \<chi>;
-      return_pmf \<lparr>state_k = k + 1, state_\<chi> = \<chi>\<rparr>
+      return_pmf \<lparr>state_p = p*f, state_\<chi> = \<chi>\<rparr>
     } else
       return_pmf \<sigma>
     }\<close>
@@ -142,9 +138,7 @@ definition run_steps :: \<open>'a list \<Rightarrow> 'a state pmf\<close> where
 
 text \<open>Line 11:\<close>
 definition estimate :: \<open>'a state \<Rightarrow> real\<close> where
-  \<open>estimate \<sigma> = card (state_\<chi> \<sigma>) / f^state_k \<sigma>\<close>
-
-definition \<open>state_p \<sigma> = f ^ state_k \<sigma>\<close>
+  \<open>estimate \<sigma> = card (state_\<chi> \<sigma>) / state_p \<sigma>\<close>
 
 lemma run_steps_snoc: \<open>run_steps (xs @[x]) = run_steps xs \<bind> step_1 x \<bind> step_2\<close>
   unfolding run_steps_def foldM_pmf_snoc by (simp add:bind_assoc_pmf)
@@ -206,6 +200,21 @@ lemma state_\<chi>_finite: \<open>AE \<sigma> in run_state_pmf \<rho>. finite (s
   using finite_subset[OF _ finite_run_state_set]
   by (intro AE_mp[OF state_\<chi>_run_state_pmf AE_I2]) auto
 
+lemma state_p_range: \<open>AE \<sigma> in run_state_pmf \<rho>. state_p \<sigma> \<in> {0<..1}\<close>
+proof (induction \<rho> rule:run_state_induct)
+  case 1 thus ?case by (simp add:run_steps_def AE_measure_pmf_iff initial_state_def)
+next
+  case (2 xs x)
+  then show ?case by (simp add:AE_measure_pmf_iff Let_def step_1_def)
+next
+  case (3 xs x)
+  let ?p = \<open>run_state_pmf (IntermState xs x)\<close>
+  have b: \<open>run_state_pmf (FinalState (xs@[x])) = ?p \<bind> step_2\<close>
+    by (simp add:run_steps_snoc)
+  have \<open>x * f \<le> 1\<close> if \<open>x \<in> {0<..1}\<close> for x using f_range that by (intro mult_le_one) auto
+  thus ?case unfolding b using 3 f_range by (simp add:AE_measure_pmf_iff step_2_def Let_def)
+qed
+
 text \<open>Lemma~\ref{le:prob_invariant}:\<close>
 lemma run_steps_preserves_expectation_le:
   fixes \<phi> :: \<open>real \<Rightarrow> bool \<Rightarrow> real\<close>
@@ -213,7 +222,7 @@ lemma run_steps_preserves_expectation_le:
     \<open>\<And> x b. \<lbrakk>0 < x; x \<le> 1\<rbrakk> \<Longrightarrow> \<phi> x b \<ge> 0\<close>
     \<open>\<And> p x. \<lbrakk>0 < p; p \<le> 1; 0 < x; x \<le> 1\<rbrakk> \<Longrightarrow> (\<integral>\<omega>. \<phi> x \<omega> \<partial>bernoulli_pmf p) \<le> \<phi> (x / p) True\<close>
     \<open>mono_on {0..1} (\<lambda>x. \<phi> x False)\<close>
-  defines \<open>aux \<equiv> \<lambda> S \<sigma>. (\<Prod> x \<in> S. \<phi> (f ^ state_k \<sigma>) (x \<in> state_\<chi> \<sigma>))\<close>
+  defines \<open>aux \<equiv> \<lambda> S \<sigma>. (\<Prod> x \<in> S. \<phi> (state_p \<sigma>) (x \<in> state_\<chi> \<sigma>))\<close>
   assumes \<open>S \<subseteq> run_state_set \<rho>\<close>
   shows \<open>measure_pmf.expectation (run_state_pmf \<rho>) (aux S) \<le> \<phi> 1 True ^ card S\<close>
   using assms(5)
@@ -238,20 +247,22 @@ next
     if \<open>\<tau> \<in> set_pmf (run_steps xs)\<close> for \<tau>
   proof(cases \<open>x \<in> S\<close>)
     case True
-    hence \<open>?L = measure_pmf.expectation (bernoulli_pmf (f ^ state_k \<tau>)) (\<lambda>x. \<phi> (f ^ state_k \<tau>) x)\<close>
-      unfolding step_1_def Let_def map_pmf_def[symmetric] integral_map_pmf aux_def
+    have p_range: \<open>state_p \<tau> \<in> {0<..1}\<close>
+      using state_p_range[where \<rho>=\<open>FinalState xs\<close>] that by (auto simp: AE_measure_pmf_iff)
+    have \<open>?L = measure_pmf.expectation (bernoulli_pmf (state_p \<tau>)) (\<lambda>x. \<phi> (state_p \<tau>) x)\<close>
+      unfolding step_1_def Let_def map_pmf_def[symmetric] integral_map_pmf aux_def using True
       by (intro integral_cong_AE AE_pmfI) simp_all
-    also have \<open>\<dots> \<le> \<phi> (f ^ state_k \<tau> / f ^ state_k \<tau>) True\<close>
-      using f_range by (intro phi(2) power_le_one zero_less_power) auto
-    also have \<open>\<dots> \<le> \<phi> 1 True\<close> using f_range by (simp add:divide_simps)
+    also have \<open>\<dots> \<le> \<phi> (state_p \<tau> / state_p \<tau>) True\<close> using p_range by (intro phi(2)) auto
+    also have \<open>\<dots> \<le> \<phi> 1 True\<close> using p_range by simp
     also have \<open>\<dots> = \<phi> 1 True ^ card (S \<inter> {x})\<close> using True by simp
     finally show ?thesis by simp
   next
     case False thus ?thesis by (simp add:aux_def)
   qed
 
-  have d: \<open>aux (S-{x}) \<tau> \<ge> 0\<close> for \<tau>
-    using f_range unfolding aux_def by (intro prod_nonneg phi(1) power_le_one) auto
+  have d: \<open>aux (S-{x}) \<tau> \<ge> 0\<close> if \<open>\<tau> \<in> set_pmf (run_steps xs)\<close> for \<tau>
+    using state_p_range[where \<rho>=\<open>FinalState xs\<close>] that unfolding aux_def
+    by (intro prod_nonneg phi(1) power_le_one) (auto simp: AE_measure_pmf_iff)
 
   have \<open>(\<integral>\<tau>. aux S \<tau> \<partial>(bind_pmf (run_steps xs) (step_1 x))) =
     (\<integral>\<tau>. (\<integral>u. aux (S - {x}) \<tau> * aux (S \<inter> {x}) u \<partial>step_1 x \<tau>) \<partial>run_steps xs)\<close>
@@ -285,41 +296,42 @@ next
   have b:\<open>finite (set_pmf (p \<bind> step_2))\<close>
     using finite_run_state_pmf[where \<rho>=\<open>FinalState (xs@[x])\<close>] a by simp
 
-  have c: \<open>(\<integral>u. (\<Prod>s\<in>S. \<phi> (f * f ^ state_k \<tau>) (s \<in> u)) \<partial>subsample (state_\<chi> \<tau>)) \<le> aux S \<tau>\<close>
-    (is \<open>?L \<le> ?R\<close>) if that': \<open>card(state_\<chi> \<tau>) = thresh\<close> for \<tau>
+  have c: \<open>(\<integral>u. (\<Prod>s\<in>S. \<phi> (f * state_p \<tau>) (s \<in> u)) \<partial>subsample (state_\<chi> \<tau>)) \<le> aux S \<tau>\<close>
+    (is \<open>?L \<le> ?R\<close>) if that': \<open>card(state_\<chi> \<tau>) = thresh\<close> \<open>\<tau> \<in> set_pmf p\<close> for \<tau>
   proof -
     let ?q = \<open>subsample (state_\<chi> \<tau>)\<close>
     let ?U = \<open>state_\<chi> \<tau>\<close>
 
-    define k' where \<open>k' = state_k \<tau>+1\<close>
+    define p' where \<open>p' = f * state_p \<tau>\<close>
 
     have d: \<open>y \<subseteq> state_\<chi> \<tau>\<close> if \<open>y \<in> set_pmf (subsample (state_\<chi> \<tau>))\<close> for y
-      using subsample[OF that'] that by auto
+      using subsample[OF that'(1)] that by auto
 
-    have e: \<open>f ^ k' \<in> {0<..1}\<close> using f_range by (auto intro:power_le_one)
-    have f: \<open>f ^ state_k \<tau> \<in> {0<..1}\<close> using f_range by (auto intro:power_le_one)
+    have e: \<open>state_p \<tau> \<in> {0<..1}\<close>
+      using that(2) unfolding p_def using state_p_range by (meson AE_measure_pmf_iff)
+    hence f: \<open>p' \<in> {0<..1}\<close> unfolding p'_def using f_range by (auto intro:mult_le_one)
 
-    have \<open>?L = (\<integral>u. (\<Prod>s\<in>(S-?U) \<union> (S\<inter>?U). \<phi> (f^k') (s\<in>u)) \<partial>?q)\<close>
-      unfolding k'_def using fin_S by (intro integral_cong_AE prod.cong AE_pmfI) auto
-    also have \<open>\<dots> = (\<integral>u. (\<Prod>s\<in>S-?U. \<phi> (f^k') (s\<in>u)) * (\<Prod>s\<in>(S\<inter>?U). \<phi> (f^k') (s\<in>u)) \<partial>?q)\<close>
+    have \<open>?L = (\<integral>u. (\<Prod>s\<in>(S-?U) \<union> (S\<inter>?U). \<phi> p' (s\<in>u)) \<partial>?q)\<close>
+      using fin_S p'_def by (intro integral_cong_AE prod.cong AE_pmfI) auto
+    also have \<open>\<dots> = (\<integral>u. (\<Prod>s\<in>S-?U. \<phi> p' (s\<in>u)) * (\<Prod>s\<in>(S\<inter>?U). \<phi> p' (s\<in>u)) \<partial>?q)\<close>
       using fin_S by (subst prod.union_disjoint) auto
-    also have \<open>\<dots> = (\<integral>u. (\<Prod>s\<in>S-?U. \<phi> (f^k') False) * (\<Prod>s\<in>(S\<inter>?U). \<phi>(f^k') (s\<in>u)) \<partial>?q)\<close>
+    also have \<open>\<dots> = (\<integral>u. (\<Prod>s\<in>S-?U. \<phi> p' False) * (\<Prod>s\<in>(S\<inter>?U). \<phi> p' (s\<in>u)) \<partial>?q)\<close>
       using d by (intro integral_cong_AE AE_pmfI arg_cong2[where f=\<open>(*)\<close>] prod.cong
           arg_cong2[where f=\<open>\<phi>\<close>]) auto
-    also have \<open>\<dots> = (\<Prod>s\<in>S-?U. \<phi> (f^k') False) * (\<integral>u. (\<Prod>s\<in>S\<inter>?U. \<phi> (f^k') (s\<in>u)) \<partial>?q)\<close>
+    also have \<open>\<dots> = (\<Prod>s\<in>S-?U. \<phi> p' False) * (\<integral>u. (\<Prod>s\<in>S\<inter>?U. \<phi> p' (s\<in>u)) \<partial>?q)\<close>
       by simp
-    also have \<open>\<dots> \<le> (\<Prod>s\<in>S-?U. \<phi> (f^k') False) * (\<Prod>s\<in>S\<inter>?U. (\<integral>u. \<phi> (f^k') u \<partial>bernoulli_pmf f))\<close>
-      using that e by (intro mult_left_mono subsample_inequality prod_nonneg) (auto intro!:phi(1))
-    also have \<open>\<dots> \<le> (\<Prod>s\<in>S-?U. \<phi> (f^k') False) * (\<Prod>s\<in>S\<inter>?U. \<phi> (f^k'/f) True)\<close>
-      using e f_range
+    also have \<open>\<dots> \<le> (\<Prod>s\<in>S-?U. \<phi> p' False) * (\<Prod>s\<in>S\<inter>?U. (\<integral>u. \<phi> p' u \<partial>bernoulli_pmf f))\<close>
+      using that f by (intro mult_left_mono subsample_inequality prod_nonneg) (auto intro!:phi(1))
+    also have \<open>\<dots> \<le> (\<Prod>s\<in>S-?U. \<phi> p' False) * (\<Prod>s\<in>S\<inter>?U. \<phi> (p'/f) True)\<close>
+      using f f_range
       by (intro mult_left_mono prod_mono phi(2) conjI integral_nonneg_AE AE_pmfI phi(1) prod_nonneg)
          auto
-    also have \<open>\<dots> \<le> (\<Prod>s\<in>S-?U. \<phi> (f^state_k \<tau>) False) * (\<Prod>s\<in>S\<inter>?U. \<phi> (f^state_k \<tau>) True)\<close>
-      using e f f_range unfolding k'_def
+    also have \<open>\<dots> \<le> (\<Prod>s\<in>S-?U. \<phi> (state_p \<tau>) False) * (\<Prod>s\<in>S\<inter>?U. \<phi> (state_p \<tau>) True)\<close>
+      using e f f_range unfolding p'_def
       by (intro mult_mono prod_mono conjI phi(1) mono_onD[OF phi(3)] prod_nonneg power_le_one) auto
-    also have \<open>\<dots> = (\<Prod>s\<in>S-?U. \<phi>(f^state_k \<tau>) (s \<in> ?U)) * (\<Prod>s\<in>S\<inter>?U. \<phi>(f^state_k \<tau>) (s \<in> ?U))\<close>
+    also have \<open>\<dots> = (\<Prod>s\<in>S-?U. \<phi>(state_p \<tau>) (s \<in> ?U)) * (\<Prod>s\<in>S\<inter>?U. \<phi>(state_p \<tau>) (s \<in> ?U))\<close>
       by simp
-    also have \<open>\<dots> = (\<Prod>s\<in>(S-?U)\<union>(S\<inter>?U). \<phi>(f^state_k \<tau>) (s \<in> ?U))\<close>
+    also have \<open>\<dots> = (\<Prod>s\<in>(S-?U)\<union>(S\<inter>?U). \<phi>(state_p \<tau>) (s \<in> ?U))\<close>
       using fin_S by (subst prod.union_disjoint[symmetric]) (auto)
     also have \<open>\<dots> = aux S \<tau>\<close> unfolding aux_def by (intro prod.cong) auto
     finally show ?thesis by simp
@@ -329,9 +341,9 @@ next
     unfolding a by simp
   also have \<open>\<dots> = (\<integral>\<tau>. (\<integral>u. aux S u \<partial>step_2 \<tau>) \<partial>p)\<close> by (intro integral_bind_pmf bounded_finite b)
   also have \<open>\<dots> = (\<integral>\<tau>. (if card(state_\<chi> \<tau>) = thresh then
-    (\<integral>u. (\<Prod>s\<in>S. \<phi> (f * f ^ state_k \<tau>) (s \<in> u)) \<partial>subsample (state_\<chi> \<tau>)) else aux S \<tau>) \<partial>p)\<close>
+    (\<integral>u. (\<Prod>s\<in>S. \<phi> (f * state_p \<tau>) (s \<in> u)) \<partial>subsample (state_\<chi> \<tau>)) else aux S \<tau>) \<partial>p)\<close>
     unfolding step_2_def map_pmf_def[symmetric] Let_def aux_def
-    by (simp add:if_distrib if_distribR cong:if_cong)
+    by (simp add:if_distrib if_distribR ac_simps cong:if_cong)
   also have \<open>\<dots> \<le> (\<integral>\<tau>. (if card(state_\<chi> \<tau>) < thresh then aux S \<tau> else aux S \<tau>) \<partial>p)\<close>
     using c by (intro integral_mono_AE AE_pmfI) auto
   also have \<open>\<dots> = (\<integral>\<tau>. aux S \<tau> \<partial>p)\<close> by simp
@@ -374,7 +386,7 @@ proof -
   have \<phi>_3: \<open>\<phi> x False \<le> \<phi> y False\<close> if \<open>x \<le> y\<close> for x y
      using that by (auto intro:h(4) simp add:\<phi>_def)
 
-  have \<open>?L = (\<integral>\<tau>. (\<Prod>x\<in>S. \<phi> (f ^ state_k \<tau>) (x \<in> state_\<chi> \<tau>)) \<partial>run_state_pmf \<rho>)\<close>
+  have \<open>?L = (\<integral>\<tau>. (\<Prod>x\<in>S. \<phi> (state_p \<tau>) (x \<in> state_\<chi> \<tau>)) \<partial>run_state_pmf \<rho>)\<close>
     unfolding \<phi>_def by (simp add:state_p_def aux_def)
   also have \<open>\<dots> \<le> \<phi> 1 True^ card S\<close> using \<phi>_1 \<phi>_2 \<phi>_3
     by (intro run_steps_preserves_expectation_le assms ) (auto intro:mono_onI)
@@ -538,53 +550,34 @@ proof -
 qed
 
 text \<open>Lemma~\ref{le:low_p}:\<close>
-lemma low_p: \<open>measure (run_steps xs) {\<sigma>. state_p \<sigma> < q} \<le> real (length xs) * exp(-real thresh/12)\<close>
+lemma low_p:
+  shows \<open>measure (run_steps xs) {\<sigma>. state_p \<sigma> < q} \<le> real (length xs) * exp(-real thresh/12)\<close>
+    (is \<open>?L \<le> ?R\<close>)
 proof -
   define \<rho> where \<open>\<rho> = FinalState xs\<close>
 
-  define j where \<open>j = nat \<lfloor>log f q\<rfloor>\<close>
-
-  have f_range': \<open>f \<ge> 0\<close> \<open>f \<le> 1\<close> using f_range by auto
-
-  have \<open>q = f powr (log f q)\<close>
-    using f_range q_range by (intro powr_log_cancel[symmetric]) auto
-  also have \<open>\<dots> \<le> f powr (\<lfloor>log f q\<rfloor>)\<close> using f_range by (intro powr_mono') auto
-  also have \<open>\<dots> \<le> f powr (real (nat \<lfloor>log f q\<rfloor>))\<close> using f_range q_range
-    by (subst of_nat_int_floor) (auto intro:divide_nonpos_neg simp add:log_def)
-  also have \<open>\<dots> = f ^ j\<close> using f_range unfolding j_def by (subst powr_realpow) auto
-  finally have f_1: \<open>q \<le> f^j\<close> by simp
-
-  have \<open>f^(j+1) = f powr (real (nat \<lfloor>log f q\<rfloor>+1))\<close>
-    unfolding j_def using f_range by (subst powr_realpow) auto
-  also have \<open>\<dots> \<le> f powr (log f q)\<close> by (intro powr_mono' f_range') linarith+
-  also have \<open>\<dots> = q\<close> using f_range q_range by (intro powr_log_cancel) auto
-  finally have f_2: \<open>f^(j+1) \<le> q\<close> by simp
-
-  have \<open>2 * real (card (set xs)) * f^j \<le> 4*f* real (card (set xs)) * f^j\<close>
-    using f_range by (intro mult_right_mono) auto
-  also have \<open>\<dots> = 4 * real (card (set xs)) * f^(j+1)\<close> by simp
-  also have \<open>\<dots> \<le> 4 * real (card (set xs)) * q\<close> using f_2 by (intro mult_left_mono) auto
-  also have \<open>\<dots> = thresh\<close> using thresh_gt_0 set_larger_than_threshold unfolding q_def by auto
-  finally have f_3: \<open>2 * real (card (set xs)) * f^j \<le> thresh\<close> by simp
-
   have ih: \<open>run_state_set \<rho> \<subseteq> set xs\<close> unfolding \<rho>_def by simp
 
-  have \<open>n > j\<close> if \<open>f^n < q\<close> for n
-    unfolding not_le[symmetric] using that f_1 power_decreasing[OF _ f_range'] by force
-  hence \<open>measure (run_steps xs) {\<omega>. state_p \<omega> < q} \<le> measure (run_state_pmf \<rho>) {\<omega>. state_k \<omega> > j}\<close>
-    unfolding \<rho>_def run_state_pmf.simps by (intro pmf_mono) (auto simp:state_p_def)
+  have \<open>?L = measure (run_state_pmf \<rho>) {\<omega>. state_p \<omega> < q}\<close>
+    unfolding \<rho>_def run_state_pmf.simps by simp
   also have \<open>\<dots> \<le> real (len_run_state \<rho>) * exp(- real thresh/12)\<close>
     using ih
   proof (induction \<rho> rule:run_state_induct)
     case 1
-    then show ?case using q_range by (simp add:run_steps_def state_p_def initial_state_def)
+    then show ?case using q_range by (simp add:run_steps_def initial_state_def)
   next
     case (2 ys x)
-    have \<open>measure (step_1 x s) {\<omega>. state_k \<omega> > j} = indicator {\<omega>. state_k \<omega> > j} s\<close>
-      for s :: \<open>'a state\<close>
-      by (simp add:step_1_def map_pmf_def[symmetric] Let_def)
+    let ?pmf = \<open>(run_state_pmf (IntermState ys x))\<close>
+    have a:\<open>run_state_set (FinalState ys) \<subseteq> set xs\<close> using 2(2) by auto
 
-    thus ?case using 2 by (simp add:measure_bind_pmf)
+    have \<open>measure ?pmf {\<omega>. state_p \<omega> < q} = (\<integral>\<sigma>. of_bool (state_p \<sigma> < q) \<partial>run_steps ys)\<close>
+      unfolding run_state_pmf.simps step_1_def Let_def by (simp add:measure_bind_pmf indicator_def)
+    also have \<open>\<dots> = (\<integral>\<sigma>. indicator {\<omega>. (state_p \<omega> < q)} \<sigma> \<partial>run_steps ys)\<close>
+      by (intro integral_cong_AE AE_pmfI) simp_all
+    also have \<open>\<dots> = measure (run_steps ys) {\<omega>. (state_p \<omega> < q)}\<close> by simp
+    also have \<open>\<dots> \<le> real (len_run_state (IntermState ys x)) * exp (- real thresh / 12)\<close>
+      using 2(1)[OF a] by simp
+    finally show ?case by simp
   next
     case (3 ys x)
     define p where \<open>p = run_state_pmf (IntermState ys x)\<close>
@@ -592,41 +585,48 @@ proof -
     have \<open>finite (set_pmf p)\<close> unfolding p_def by (intro finite_run_state_pmf)
     note [simp] = integrable_measure_pmf_finite[OF this]
 
-    have a: \<open>run_state_pmf (FinalState (ys@[x])) = p \<bind> step_2\<close>
+    have a: \<open>run_state_pmf (FinalState (ys@[x])) = p \<bind> step_2\<close> (is \<open>?pmf= _\<close>)
       by (simp add:run_steps_snoc p_def)
 
     have b: \<open>run_state_set (IntermState ys x) \<subseteq> set xs\<close>
       using 3(2) by simp
 
-    have c:\<open>measure (step_2 \<sigma>) {\<sigma>. state_k \<sigma> > j} \<le>
-      indicator {\<sigma>. state_k \<sigma> > j \<or> card (state_\<chi> \<sigma>) \<ge> thresh \<and> state_k \<sigma> = j} \<sigma>\<close>
-      for j and \<sigma> :: \<open>'a state\<close>
-      by (simp add:step_2_def Let_def indicator_def map_pmf_def[symmetric])
-
-    have d:\<open>measure (step_2 \<sigma>) {\<sigma>. state_p \<sigma> < q} \<le>
-      indicator {\<sigma>. state_p \<sigma> < q \<or> card (state_\<chi> \<sigma>) \<ge> thresh} \<sigma>\<close>
+    have c:\<open>measure (step_2 \<sigma>) {\<sigma>. state_p \<sigma> < q} \<le>
+      indicator {\<sigma>. state_p \<sigma> < q \<or> (card (state_\<chi> \<sigma>) = thresh \<and> state_p \<sigma> \<in> {q..<q/f}) } \<sigma>\<close>
       for \<sigma> :: \<open>'a state\<close>
-      by (simp add:step_2_def Let_def indicator_def)
+      using f_range
+      by (simp add:step_2_def Let_def indicator_def map_pmf_def[symmetric] divide_simps)
 
-    have \<open>measure p {\<sigma>. card (state_\<chi> \<sigma>) \<ge> thresh \<and> state_k \<sigma> = j} \<le>
+    have d: \<open>2 * real (card (set xs)) \<le> real thresh / \<alpha>\<close> if \<open>\<alpha> \<in> {q..<q / f}\<close> for \<alpha>
+    proof -
+      have \<open>\<alpha> \<le> q * (1/f)\<close> using that by simp
+      also have \<open>\<dots> \<le> q * 2\<close> using q_range f_range by (intro mult_left_mono) (auto simp:divide_simps)
+      finally have \<open>\<alpha> \<le> 2*q\<close> by simp
+      hence \<open>\<alpha> \<le> real thresh / (2 * real (card (set xs)))\<close>
+        using set_larger_than_threshold thresh_gt_0 unfolding q_def by (simp add:divide_simps)
+      thus ?thesis
+        using set_larger_than_threshold thresh_gt_0 that q_range by (simp add:field_simps)
+    qed
+
+    hence \<open>measure p {\<sigma>. card (state_\<chi> \<sigma>) = thresh \<and> state_p \<sigma> \<in> {q..<q/f}} \<le>
       measure p {\<sigma>. (1+1) * real(card(set xs)) \<le> estimate \<sigma> \<and> q \<le> state_p \<sigma>}\<close>
-      using f_1 f_3 f_range by (intro pmf_mono) (simp add:estimate_def state_p_def field_simps)
+      unfolding estimate_def by (intro pmf_mono) (simp add:estimate_def)
     also have \<open>\<dots> \<le> exp (- real thresh / 12 * 1^2)\<close>
       unfolding p_def by (intro upper_tail_bound b) simp
     finally have e:
-      \<open>measure p {\<sigma>. card (state_\<chi> \<sigma>) \<ge> thresh \<and> state_k \<sigma> = j} \<le> exp (- real thresh / 12)\<close>
+      \<open>measure p {\<sigma>. card (state_\<chi> \<sigma>) = thresh \<and> state_p \<sigma> \<in> {q..<q/f}} \<le> exp (- real thresh / 12)\<close>
       by simp
 
-    have \<open>measure (run_state_pmf (FinalState (ys @ [x]))) {\<omega>. state_k \<omega> > j} =
-      (\<integral>s. measure (step_2 s) {\<omega>. state_k \<omega> > j} \<partial>p)\<close>
+    have \<open>measure (run_state_pmf (FinalState (ys @ [x]))) {\<omega>. state_p \<omega> < q} =
+      (\<integral>s. measure (step_2 s) {\<omega>. state_p \<omega> < q} \<partial>p)\<close>
       unfolding a by (simp add:measure_bind_pmf)
-    also have \<open>\<dots> \<le> (\<integral>s. indicator {\<omega>. state_k \<omega>>j \<or> card(state_\<chi> \<omega>) \<ge> thresh \<and> state_k \<omega>=j} s \<partial>p)\<close>
+    also have \<open>\<dots> \<le> (\<integral>s. indicator {\<omega>. state_p \<omega> < q \<or> card (state_\<chi> \<omega>) = thresh \<and> state_p \<omega> \<in> {q..<q/f}} s \<partial>p)\<close>
       by (intro integral_mono_AE AE_pmfI c) simp_all
-    also have \<open>\<dots> = measure p {\<omega>. state_k \<omega> > j \<or> card (state_\<chi> \<omega>) \<ge> thresh \<and> state_k \<omega> = j}\<close>
+    also have \<open>\<dots> = measure p {\<omega>. state_p \<omega> < q \<or> card (state_\<chi> \<omega>) = thresh \<and> state_p \<omega> \<in> {q..<q/f}}\<close>
       by simp
     also have \<open>\<dots> \<le>
-      measure p {\<omega>. state_k \<omega> > j} +
-      measure p {\<omega>. card (state_\<chi> \<omega>) \<ge> thresh \<and> state_k \<omega> = j}\<close>
+      measure p {\<omega>. state_p \<omega> < q} +
+      measure p {\<omega>. card (state_\<chi> \<omega>) = thresh \<and> state_p \<omega> \<in> {q..<q/f}}\<close>
       by (intro pmf_add) auto
     also have \<open>\<dots> \<le> length ys * exp (- real thresh / 12) + exp (- real thresh / 12)\<close>
       using 3(1)[OF b] by (intro add_mono e) (simp add:p_def)
@@ -818,7 +818,7 @@ end
 
 lemma deterministic_phase:
   assumes \<open>card (run_state_set \<sigma>) < thresh\<close>
-  shows \<open>run_state_pmf \<sigma> = return_pmf \<lparr> state_k = 0, state_\<chi> = run_state_set \<sigma> \<rparr>\<close>
+  shows \<open>run_state_pmf \<sigma> = return_pmf \<lparr> state_p = 1, state_\<chi> = run_state_set \<sigma> \<rparr>\<close>
   using assms
 proof (induction \<sigma> rule:run_state_induct)
   case 1 thus ?case by (simp add:run_steps_def initial_state_def)
@@ -851,28 +851,28 @@ proof (cases \<open>card (set xs) \<ge> thresh\<close>)
     unfolding A_def by (intro correctness_aux True assms)
 next
   case False
-  hence \<open>run_steps xs = return_pmf \<lparr> state_k = 0, state_\<chi> = (set xs) \<rparr>\<close>
+  hence \<open>run_steps xs = return_pmf \<lparr> state_p = 1, state_\<chi> = (set xs) \<rparr>\<close>
     using deterministic_phase[where \<sigma>=\<open>FinalState xs\<close>] by simp
-  thus ?thesis using assms(1,2) by (simp add:indicator_def state_p_def estimate_def A_def not_less)
+  thus ?thesis using assms(1,2) by (simp add:indicator_def estimate_def A_def not_less)
 qed
 
-lemma state_k_run_state_pmf:
+lemma p_pos:
   fixes \<rho> :: \<open>'a run_state\<close>
-  shows \<open>AE \<omega> in run_state_pmf \<rho>. state_k \<omega> \<le> len_run_state \<rho>\<close>
-proof (induction \<rho> rule:run_state_induct)
-  case 1 thus ?case by (simp add:run_steps_def AE_measure_pmf_iff initial_state_def)
-next
-  case (2 xs x)
-  then show ?case by (simp add:AE_measure_pmf_iff step_1_def Let_def remove_def)
-next
-  case (3 xs x)
-  let ?p = \<open>run_state_pmf (IntermState xs x)\<close>
-  have \<open>run_state_pmf (FinalState (xs@[x])) = ?p \<bind> step_2\<close>
-    by (simp add:run_steps_snoc)
+  shows \<open>\<exists>M\<in>{0<..1}. AE \<omega> in run_steps xs. state_p \<omega> \<ge> M\<close>
+proof -
+  have fin:\<open>finite (set_pmf (run_steps xs))\<close>
+    using finite_run_state_pmf[where \<rho>=\<open>FinalState xs\<close>] by simp
+  define M where \<open>M = (MIN \<sigma> \<in> set_pmf (run_steps xs). state_p \<sigma>)\<close>
+  have \<open>M \<in> state_p ` set_pmf (run_steps xs)\<close>
+    using fin set_pmf_not_empty unfolding M_def by (intro Min_in) auto
+  also have \<open>\<dots> \<subseteq> {0<..1}\<close>
+    using state_p_range[where \<rho>=\<open>FinalState xs\<close>]
+    by (intro image_subsetI) (simp add:AE_measure_pmf_iff)
+  finally have \<open>M \<in> {0<..1}\<close> by simp
 
-  thus ?case using 3
-    apply (simp add:AE_measure_pmf_iff step_2_def Let_def)
-    using le_SucI by blast
+  moreover have \<open>AE \<omega> in run_steps xs. state_p \<omega> \<ge> M\<close>
+    using fin unfolding AE_measure_pmf_iff M_def by (intro ballI Min_le) auto
+  ultimately show ?thesis by auto
 qed
 
 lemma run_steps_expectation_sing:
@@ -884,43 +884,33 @@ proof -
     using finite_run_state_pmf[where \<rho>=\<open>FinalState xs\<close>] by simp
   note int = integrable_measure_pmf_finite[OF this]
 
-  define Mi where \<open>Mi = f ^ len_run_state (FinalState xs)\<close>
-
-  have Mi:\<open>0 < Mi\<close> \<open>Mi \<le> 1\<close>
-    unfolding Mi_def using f_range by (auto simp add: power_le_one)
-  have \<open>AE \<sigma> in run_state_pmf (FinalState xs). Mi \<le> state_p \<sigma>\<close>
-    apply (subst AE_mp[OF state_k_run_state_pmf])
-    unfolding Mi_def state_p_def
-    using f_range by (auto intro!: power_decreasing)
-  then have *: \<open>AE \<sigma> in run_steps xs. Mi \<le> state_p \<sigma>\<close>
-    by (metis run_state_pmf.simps(1))
+  obtain M where *: \<open>AE \<sigma> in run_steps xs. M \<le> state_p \<sigma>\<close> and M_range: \<open>M \<in> {0<..1}\<close>
+    using p_pos by blast
   then have \<open>(\<integral>\<omega>. of_bool (i \<in> state_\<chi> \<omega>) / state_p \<omega> \<partial>run_steps xs) =
-    (\<integral>\<tau>. (\<Prod>x\<in>{i}. of_bool (Mi \<le> state_p \<tau>) * (of_bool (x \<in> state_\<chi> \<tau>) / state_p \<tau>))
+    (\<integral>\<tau>. (\<Prod>x\<in>{i}. of_bool (M \<le> state_p \<tau>) * (of_bool (x \<in> state_\<chi> \<tau>) / state_p \<tau>))
       \<partial>run_state_pmf (FinalState xs))\<close>
     by (auto intro!: integral_cong_AE)
 
   also have \<open>\<dots> \<le> 1 ^ card {i}\<close>
-    apply (intro run_steps_preserves_expectation_le'[OF Mi])
-    using i unfolding concave_on_iff by auto
+    using M_range i by (intro run_steps_preserves_expectation_le') (auto simp:concave_on_iff)
   finally have
     le: \<open>?L \<le> 1\<close> by auto
 
-  have concave: \<open>concave_on {0..1 / Mi} ((-) (1 / Mi + 1))\<close>
+  have concave: \<open>concave_on {0..1 / M} ((-) (1 / M + 1))\<close>
     unfolding concave_on_iff
-    using Mi apply (clarsimp simp add: field_simps)
+    using M_range apply (clarsimp simp add: field_simps)
     by (metis combine_common_factor distrib_right linear mult_1_left)
 
-  have \<open>1 / Mi + 1 - (\<integral>\<omega>. of_bool (i \<in> state_\<chi> \<omega>) / state_p \<omega> \<partial>run_steps xs) =
-    (\<integral>\<omega>. 1 / Mi + 1 - of_bool (i \<in> state_\<chi> \<omega>) / state_p \<omega> \<partial>run_steps xs) \<close>
+  have \<open>1 / M + 1 - (\<integral>\<omega>. of_bool (i \<in> state_\<chi> \<omega>) / state_p \<omega> \<partial>run_steps xs) =
+    (\<integral>\<omega>. 1 / M + 1 - of_bool (i \<in> state_\<chi> \<omega>) / state_p \<omega> \<partial>run_steps xs) \<close>
     apply (subst Bochner_Integration.integral_diff)
     using int by auto
-  also have \<open>\<dots> = (\<integral>\<tau>. (\<Prod>x\<in>{i}. of_bool (Mi \<le> state_p \<tau>) *
-    (1 / Mi + 1 - of_bool (x \<in> state_\<chi> \<tau>) / state_p \<tau>)) \<partial>run_state_pmf (FinalState xs))\<close>
+  also have \<open>\<dots> = (\<integral>\<tau>. (\<Prod>x\<in>{i}. of_bool (M \<le> state_p \<tau>) *
+    (1 / M + 1 - of_bool (x \<in> state_\<chi> \<tau>) / state_p \<tau>)) \<partial>run_state_pmf (FinalState xs))\<close>
     using * by (auto intro!: integral_cong_AE)
-  also have \<open>\<dots> \<le> (1 / Mi + 1 - 1) ^ card {i}\<close>
-    apply (intro run_steps_preserves_expectation_le'[OF Mi concave])
-    using i Mi by (auto simp add: field_simps)
-  also have \<open>\<dots> = 1 / Mi\<close> by auto
+  also have \<open>\<dots> \<le> (1 / M + 1 - 1) ^ card {i}\<close>
+    using i M_range by (intro run_steps_preserves_expectation_le'[OF _ _ concave]) (auto simp: field_simps)
+  also have \<open>\<dots> = 1 / M\<close> by auto
   finally have ge:\<open> -(\<integral>\<sigma>. of_bool (i \<in> state_\<chi> \<sigma>) / state_p \<sigma> \<partial>run_steps xs) \<le> -1\<close> by auto
   show ?thesis using le ge by auto
 qed
